### [Convert to Base -2](https://leetcode.com/problems/convert-to-base-2)

<p>Given a number <code>N</code>, return a string consisting of <code>&quot;0&quot;</code>s and <code>&quot;1&quot;</code>s&nbsp;that represents its value in base <code><strong>-2</strong></code>&nbsp;(negative two).</p>

<p>The returned string must have no leading zeroes, unless the string is <code>&quot;0&quot;</code>.</p>

<p>&nbsp;</p>

<div>
<p><strong>Example 1:</strong></p>

<pre>
<strong>Input: </strong><span id="example-input-1-1">2</span>
<strong>Output: </strong><span id="example-output-1">&quot;110&quot;
<strong>Explantion:</strong> (-2) ^ 2 + (-2) ^ 1 = 2</span>
</pre>

<div>
<p><strong>Example 2:</strong></p>

<pre>
<strong>Input: </strong><span id="example-input-2-1">3</span>
<strong>Output: </strong><span id="example-output-2">&quot;111&quot;
</span><span id="example-output-1"><strong>Explantion:</strong> (-2) ^ 2 + (-2) ^ 1 + (-2) ^ 0</span><span> = 3</span>
</pre>

<div>
<p><strong>Example 3:</strong></p>

<pre>
<strong>Input: </strong><span id="example-input-3-1">4</span>
<strong>Output: </strong><span id="example-output-3">&quot;100&quot;
</span><span id="example-output-1"><strong>Explantion:</strong> (-2) ^ 2 = 4</span>
</pre>

<p>&nbsp;</p>

<p><strong><span>Note:</span></strong></p>

<ol>
	<li><span><code>0 &lt;= N &lt;= 10^9</code></span></li>
</ol>
</div>
</div>
</div>